Add requirements for Gas separator

examples/Constrained_Until.thy
@@ -129,7 +129,44 @@ always_imp s (\<lambda> s1. constrained_until2_inv t1 t2 t1_1 t2_1 A1' A2' s s1)
 lemma constrained_until2_one_point: "
 toEnvP s \<Longrightarrow>t1 = 0 \<and>A2' s s \<or> A1' s s \<and> t1_1 s = 0 \<and> t2_1 s > 0 \<Longrightarrow> constrained_until2_inv t1 t2 t1_1 t2_1 A1' A2' s s"
   unfolding constrained_until2_inv_def always_imp_def
- by (metis bot_nat_0.extremum dual_order.refl leD order_le_imp_less_or_eq toEnvNum_id)
+  by (metis bot_nat_0.extremum dual_order.refl leD order_le_imp_less_or_eq toEnvNum_id)
+
+definition constrained_until3 where "constrained_until3 t1 t2 A1 A2  s s1 \<equiv>
+toEnvNum s1 s \<ge> t2 \<longrightarrow>
+(\<exists> r2. toEnvP r2 \<and> s1 \<le> r2 \<and> r2 \<le> s \<and> toEnvNum s1 r2 \<ge> t1 \<and> toEnvNum s1 r2 \<le> t2 \<and> A2 s r2 \<and>
+(\<forall> r1. toEnvP r1 \<and> s1 \<le> r1 \<and> r1 < r2 \<longrightarrow> A1 s r1))"
+
+definition constrained_until3_inv where "constrained_until3_inv t1 t2 P1 t2_1 A1' A2' s s1 \<equiv>
+\<forall> t1_2. P1 s t1_2 \<longrightarrow>
+((\<exists> r2. toEnvP r2 \<and> s1 \<le> r2 \<and> r2 \<le> s \<and> toEnvNum s1 r2 \<ge> t1 \<and> toEnvNum s1 r2 \<le> t2 \<and> A2' s r2 \<and>
+(\<forall> r1. toEnvP r1 \<and> s1 \<le> r1 \<and> r1 < r2 \<longrightarrow> A1' s r1)) \<or>
+toEnvNum s1 s \<ge> t1_2 \<and> toEnvNum s1 s < t2_1 s \<and>
+(\<forall> r1. toEnvP r1 \<and> s1 \<le> r1 \<and> r1 \<le> s \<longrightarrow> A1' s r1))"
+
+lemma constrained_until2_rule: "
+consecutive s s' \<Longrightarrow>
+always_imp s (A1' s) (A1' s') \<and>
+always_imp s (A2' s) (A2' s') \<and>
+(\<forall> t1_2'. P1 s' t1_2' \<longrightarrow> 
+  (\<exists> t1_2. P1 s t1_2 \<and> (t2_1 s = 0 \<or>  t1_2 \<ge> t2_1 s \<or> A2' s' s' \<and> t1_2 + 1 \<ge> t1 \<and> t2_1 s \<le> t2 \<or> A1' s' s' \<and> t1_2 + 1 \<ge> t1_2' \<and> t2_1 s < t2_1 s'))) \<Longrightarrow>
+always_imp s (\<lambda> s1. constrained_until3_inv t1 t2 P1 t2_1 A1' A2' s s1) (\<lambda> s1. constrained_until3_inv t1 t2 P1 t2_1 A1' A2' s' s1)"
+  apply(unfold constrained_until3_inv_def always_imp_def)
+  unfolding less_eq_state.simps less_state.simps
+  apply(rule allI)
+  subgoal for s1
+    apply(rule impI)
+    apply(rule allI)
+    subgoal for t1_2
+      apply(erule conjE)
+      apply(rotate_tac -1)
+      apply(erule conjE)
+      apply(rotate_tac -1)
+      apply(rule impI)
+      apply(erule allE[of _ t1_2])
+      apply(rotate_tac -1)
+      apply(erule impE)
+      apply assumption
+
 
 end
  
